@@ -12,17 +12,17 @@ public structure VarWidths where
   inner: Array Nat
 deriving Repr
 
-public def VarWidths.varWidth (v: VarWidths) (index: USize) :=
-  match v.inner[index]? with
-  | some width => width
-  | none => 0
+@[expose]
+public def VarWidths.size (v: VarWidths) : Nat :=
+  v.inner.size
 
-public def VarWidths.usize (v: VarWidths) :=
-  v.inner.usize
+public def VarWidths.varWidth (v: VarWidths) (index: Fin v.size) :=
+  let h: index.val < v.inner.size := by simp[size]
+  v.inner[index.val]'h
 
 public inductive Formula (v: VarWidths): Nat → Type where
   | Constant: {w: Nat} → Bitvector w → Formula v w
-  | Variable: (i : {a: USize // a < v.usize}) → Formula v (VarWidths.varWidth v i)
+  | Variable: (i : Fin v.size) → Formula v (VarWidths.varWidth v i)
   | Unary: {w: Nat} → Formula v w → UniOp → Formula v w
   | BinaryNormal: {w: Nat} → Formula v w → Formula v w → BiNormalOp → Formula v w
   | BinaryReduction: {w: Nat} → Formula v w → Formula v w → BiReductionOp → Formula v 1
